Semestre6/metodos_num/t1_parte1.py
@@ -1,0 +1,35 @@
+import numpy as np
+import matplotlib.pyplot as plt
+from scipy import interpolate
+from collections import namedtuple
+import os
+os.environ['QT_PLUGIN_PATH'] = '/opt/anaconda3/lib'
+import videolib as vd 
+
+import sys
+
+
+# Tupla com os parametros de cada conjunto de teste.
+Videoset = namedtuple('Videoset', ['path', 'frames', 'extension'])
+
+# Videos de teste disponibilizados.
+video_sets = {
+    'OldTownCross': Videoset('OldTownCross', 500, 'jpg'),
+    'Riverbed': Videoset('Riverbed', 250, 'jpg'),
+    'Stefan': Videoset('Stefan', 300, 'jpg'),
+    'Tennis': Videoset('Tennis', 150, 'jpg'),
+}
+
+def first_interpol():
+    videoset = video_sets['OldTownCross']
+    frame_count = 0
+    for frame1, frame2 in vd.load_frames(videoset, total_frames=498):
+        print(frame_count)
+        frame_count = vd.save_frame(frame_count, frame1)
+        for i in np.linspace(0, 1, num = 4)[1:-1]:
+            print(frame_count)
+            interpol_frame = np.multiply(frame1, i) + np.multiply(frame2, 1-i)
+            frame_count = vd.save_frame(frame_count, interpol_frame)
+    
+    vd.write_video('output', 'video', 75)
+
