Semestre6/fila.dfy
@@ -1,0 +1,72 @@
+class {:autocontracts}  FilaNat
+{
+    //Implementação
+    var a: array<nat>;
+    var tail: nat;
+    //Abstração
+    ghost var Conteudo: seq<nat>;
+
+    predicate Valid()
+    {
+        a.Length != 0
+        && 0 <= tail <= a.Length
+        && a[0..tail] == Conteudo
+    }
+    constructor ()
+    ensures Conteudo == []
+    {
+        a := new nat[5];
+        tail := 0;
+        Conteudo := [];
+    }
+
+    method Tamanho() returns (n:nat)
+    ensures n == |Conteudo|
+    {
+        return tail;
+    }
+
+    method Enfileira(e:nat)
+    ensures Conteudo == old(Conteudo) + [e]
+    ensures |Conteudo| == |old(Conteudo)| + 1
+    {
+        if (tail == a.Length)
+        {
+            var b := new nat[2 * a.Length];
+            forall(i | 0 <= i < a.Length)
+            {
+                b[i] := a[i];
+            }
+            a := b;
+        }
+        a[tail] := e;
+        tail := tail + 1;
+        Conteudo := Conteudo + [e];
+    }
+
+    method Desenfileira() returns (e:nat)
+    requires |Conteudo| > 0
+    ensures e == old(Conteudo)[0]
+    ensures Conteudo == old(Conteudo)[1..]
+    ensures |Conteudo| == |old(Conteudo)| - 1
+    {
+        e := a[0];
+        tail := tail - 1;
+        forall(i | 0 <= i < tail)
+        {
+            a[i] := a[i+1];
+        }
+        Conteudo := a[0..tail];
+    }
+}
+
+method Main()
+{
+    var fila := new FilaNat();
+    fila.Enfileira(1);
+    fila.Enfileira(2);
+    assert fila.Conteudo == [1,2];
+    var e := fila.Desenfileira();
+    assert e == 1;
+    assert fila.Conteudo == [2];
+}
