Semestre6/script.sql
@@ -1,45 +1,5 @@
------ INSERTIONS -------
-
-insert into CBO2002_GRANDEGRUPO
-select * from duncanbda.CBO2002_GRANDEGRUPO;
-
-insert into CBO2002_GRUPO
-select * from duncanbda.CBO2002_GRUPO;
-
-insert into CBO2002_SUBGRUPO
-select * from duncanbda.CBO2002_SUBGRUPO;
-
-insert into CBO2002_FAMILIA
-select * from duncanbda.CBO2002_FAMILIA;
-
-insert into CBO2002_OCUPACAO
-select * from duncanbda.CBO2002_OCUPACAO;
-
-insert into CID10_CATEGORIAS
-select * from duncanbda.CID10_CATEGORIAS;
-
-insert into CID10_SUBCATEGORIAS
-select * from duncanbda.CID10_SUBCATEGORIAS;
-
-insert into CNAE20_DIVISOES
-select * from duncanbda.CNAE20_DIVISOES;
-
-insert into CNAE20_GRUPOS
-select * from duncanbda.CNAE20_GRUPOS;
-
-insert into CNAE20_CLASSES
-select * from duncanbda.CNAE20_CLASSES;
-
-insert into MUNICIPIOS
-select * from duncanbda.MUNICIPIOS;
-
-insert into MUNICIPIOS_POPULACOES
-select * from duncanbda.MUNICIPIOS_POPULACOES;
-
-insert into ACID_TRABALHO_2019_10
-select * from duncanbda.ACID_TRABALHO_2019_10;
-
-commit;
+--- Nome: Conrado Santos Boeira
+--- Matrícula: 17104100-7
 
 ---- Get Stats -----
 analyze table CBO2002_FAMILIA compute statistics;
@@ -79,7 +39,7 @@ where (AGENTE_CAUSADOR_ACIDENTE like 'Ser Vivo%' and sexo = 'Masculino' and CNAE
 order by categoria,natureza_da_lesao;
 
 
----- Create index -----
+---- Create/drop index -----
 create bitmap index bix_agente on ACID_TRABALHO_2019_10 (AGENTE_CAUSADOR_ACIDENTE);
 create bitmap index bix_sexo on ACID_TRABALHO_2019_10 (sexo);
 create bitmap index bix_classes on ACID_TRABALHO_2019_10 (CNAE20_EMPREGADOR);
@@ -95,3 +55,40 @@ create index ix_classes on ACID_TRABALHO_2019_10 (CNAE20_EMPREGADOR);
 drop index ix_agente;
 drop index ix_sexo;
 drop index ix_classes;
+
+---- Get Stats -----
+analyze table CBO2002_FAMILIA compute statistics;
+analyze table CBO2002_GRANDEGRUPO compute statistics;
+analyze table CBO2002_GRUPO compute statistics;
+analyze table CBO2002_OCUPACAO compute statistics;
+analyze table CBO2002_SUBGRUPO compute statistics;
+analyze table CID10_CATEGORIAS compute statistics;
+analyze table CID10_SUBCATEGORIAS compute statistics;
+analyze table CNAE20_CLASSES compute statistics;
+analyze table CNAE20_DIVISOES compute statistics;
+analyze table CNAE20_GRUPOS compute statistics;
+analyze table MUNICIPIOS compute statistics;
+analyze table MUNICIPIOS_POPULACOES compute statistics;
+analyze table ACID_TRABALHO_2019_10 compute statistics;
+
+select table_name, num_rows, blocks, avg_space, avg_row_len from user_tables;
+select table_name, column_id, column_name, data_type, data_length, num_distinct,
+density, num_nulls, avg_col_len from user_tab_columns;
+select table_name, constraint_name, constraint_type, search_condition, index_name
+from user_constraints;
+SELECT SEGMENT_NAME, BYTES, BLOCKS FROM USER_SEGMENTS
+ORDER BY 2 DESC;
+
+---- Queries -----
+
+select denominacao, mes_ano_acidente, count(*) as numero_acidentes
+from ACID_TRABALHO_2019_10 join CNAE20_CLASSES on CNAE20_EMPREGADOR = CLASSE_NUM
+where(AGENTE_CAUSADOR_ACIDENTE like 'Ser Vivo%' and sexo = 'Masculino' and CLASSE_NUM = 5310)
+group by denominacao, mes_ano_acidente
+order by MES_ANO_ACIDENTE, denominacao;
+
+select distinct CID10_CATEGORIAS.cat as categoria, CID10_CATEGORIAS.descricao as descricao, natureza_da_lesao
+from ACID_TRABALHO_2019_10 join CID10_SUBCATEGORIAS on ACID_TRABALHO_2019_10.cid_10 = CID10_SUBCATEGORIAS.subcat  
+join CID10_CATEGORIAS on CID10_SUBCATEGORIAS.cat = CID10_CATEGORIAS.cat
+where (AGENTE_CAUSADOR_ACIDENTE like 'Ser Vivo%' and sexo = 'Masculino' and CNAE20_EMPREGADOR = 5310)
+order by categoria,natureza_da_lesao;
